Tests.thy
@@ -3,267 +3,104 @@ theory Tests
     (* "../LTS-formalization/Datalog/Datalog"
     "AI_Planning_Languages_Semantics.PDDL_STRIPS_Semantics"
     "Verified_SAT_Based_AI_Planning.STRIPS_Representation" *)
+    "AI_Planning_Languages_Semantics.PDDL_STRIPS_Checker"
 begin
 
 text \<open>This is just a collection of random stuff. Read at your own risk.\<close>
 
-value "{(True, True)}\<^sup>*"
-
-lemma "(prod.swap ` s)\<^sup>* = prod.swap ` (s\<^sup>*)" oops
-lemma "r\<inverse> = prod.swap ` r" by auto
-lemma "(r\<inverse>)\<^sup>* = (r\<^sup>*)\<inverse>" by (rule rtrancl_converse)
-
-locale el_localo =
-  fixes types :: "(string \<times> string) list"
-
+subsection \<open> locale/context tutorial \<close>
+locale my_loc =
+  fixes x :: int
 begin
 
-definition "subtype_rel \<equiv> set (map prod.swap (types))"
-definition of_type :: "string list \<Rightarrow> string list \<Rightarrow> bool" where
-    "of_type oT T \<equiv> set oT \<subseteq> subtype_rel\<^sup>* `` set T"
+definition "evsa \<equiv> even x"
 
-value "(((\<lambda>x. None) :: int \<rightharpoonup> int set) (3 \<mapsto> {1, 2})) 3"
-value "(((\<lambda>x. 2*x) :: int \<Rightarrow> int) (3 := 4))"
 end
 
-(* alternatively, use remdups on each bag at the end *)
-fun conc_unique :: "'a list \<Rightarrow> 'a list \<Rightarrow> 'a list" where
-  "conc_unique [] rs = rs" |
-  "conc_unique (l # ls) rs = conc_unique ls (if l \<in> set rs then rs else l # rs)"
+interpretation ahsh: my_loc 6 .
 
-lemma conc_unique_set: "set (conc_unique xs ys) = set xs \<union> set ys"
-  apply (induction xs arbitrary: ys)
-  by auto
-(*fun upd_bag :: "('a \<times> 'a list) \<Rightarrow> ('a \<Rightarrow> 'a list) \<Rightarrow> ('a \<Rightarrow> 'a list)" where
-  "upd_bag (l, rs) R = R(l := conc_unique rs (R l))" *)
+value "ahsh.evsa"
 
-(* definition upd_bags :: "('a \<times> 'a list) list \<Rightarrow> ('a \<Rightarrow> 'a list) \<Rightarrow> ('a \<Rightarrow> 'a list)" where
-  "upd_bags pairs R = fold upd_bag pairs R" *)
 
-(* definition clomp where
-  "clomp keys value \<equiv> map (\<lambda>k. (k, value)) keys" *)
+context my_loc
+begin
 
-(* definition shnu where
-  "shnu rel r_ls l_rs \<equiv> upd_bags (clomp r_ls l_rs) rel" *)
+definition "cool \<equiv> x - 1"
 
-definition upd_bag :: "'a list \<Rightarrow> 'a \<Rightarrow> ('a \<Rightarrow> 'a list) \<Rightarrow> ('a \<Rightarrow> 'a list)" where
-  "upd_bag values key rel \<equiv> rel(key := conc_unique values (rel key))"
+context
+  fixes scale :: int
+begin
+definition "sc_x \<equiv> scale * x"
 
-definition upd_all where
-  "upd_all rel keys values \<equiv> fold (upd_bag values) keys rel"
+end
 
-thm upd_all_def[unfolded upd_bag_def]
-lemma upd_all_cons:
-  "upd_all rel (a#as) values = upd_all (rel(a := conc_unique values (rel a))) as values"
-  by (simp add: upd_all_def[unfolded upd_bag_def])
+end
 
-(* This is going to be weird but bear with me *)
+value "ahsh.cool"
+value "ahsh.sc_x 6"
 
-lemma
-  assumes "rel k = v" "a \<noteq> k"
-  shows "(rel (a := conc_unique values (rel a))) k = v"
-  using assms by auto
+locale my_loc2 = my_loc +
+  assumes ev: evsa
+begin
 
-lemma
-  assumes "rel k = v"
-  shows "set ((rel (k := conc_unique values (rel k))) k) = set values \<union> set (rel k)"
-  using assms conc_unique_set by (metis fun_upd_same)
+definition "hot \<equiv> x + 1"
+end
 
-(* two properties we are interested in: that f k = the original value and that after the update with k=v, f k = {values} \<union> original
-initially, f k = original. in each update step, if a=k, then result k = values + original.
-otherwise, result = original.
-*)
+interpretation lava : my_loc2 4
+  by (simp add: my_loc.evsa_def my_loc2_def)
 
-(* need some sort of inverse induction for this *)
-lemma
-  assumes "of_k_is_og y0"
-    "\<forall>y. of_k_is_og y \<longrightarrow> of_k_is_un (f k y)"
-    "\<forall>x y. of_k_is_un y \<longrightarrow> of_k_is_un (f x y)"
-    "\<forall>x y. x \<noteq> k \<and> of_k_is_og y \<longrightarrow> of_k_is_og (f x y)"
-    "k \<in> set xs"
-  shows "of_k_is_un (fold f xs y0)"
-  using assms
-proof (induction xs arbitrary: y)
-  case (Cons a as)
-    show ?case
-  proof (cases "k \<in> set as")
-    case True
-    note Cons.IH[OF assms(1) assms(2) assms(3) assms(4) this]
-    hence "of_k_is_un (fold f as y0)" .
-    oops
 
-lemma fold_induct: "\<lbrakk>P y0; \<And>x y. P y \<Longrightarrow> P (f x y)\<rbrakk> \<Longrightarrow> P (fold f xs y0)"
-  apply (induction xs arbitrary: y0)
-  by simp_all
+print_locale! my_loc2
+thm my_loc2_def
 
-lemma todo: "\<forall>k. set (conc_unique values ((upd_all rel keys values) k)) = set values \<union> set (rel k)"
+definition (in my_loc2) "sixer \<equiv> x+6"
+lemma (in my_loc2) sixer_even: "even sixer"
+  using ev evsa_def sixer_def by auto
+
+thm "lava.sixer_even"
+thm "my_loc2.sixer_even"
+
+value "lava.sixer"
+
+locale my_loc3 = my_loc2 "fst pair" for
+  pair :: "int \<times> int" +
+  assumes pair_eq: "fst pair = snd pair"
+
+locale my_loc_dos =
+  un: my_loc2 a + dos: my_loc2 b
+  for a and b +
+  assumes pair_eq: "a = b"
+begin
+
+lemma "(a + b) mod 4 = 0"
+proof -
+  have "even a"
+    using un.ev un.evsa_def by auto
   oops
 
+lemma "un.evsa" by (simp add: un.ev)
 
+end
 
-(* property is that applying conc_unique is like \<union>-ing values*)
+(* sublocale, but I'm too lazy for an example rn *)
 
-lemma fold_upd_preserves:
-  assumes "k \<notin> set keys"
-  shows "fold (\<lambda>k f. f(k := v)) keys f k = f k"
-  using assms
-  by (induction keys arbitrary: f) simp_all
+(* unique existence *)
 
-lemma
-  assumes "k \<in> set ks"
-  shows "fold (\<lambda>k f. f(k := v)) ks f k = v"
-  using assms
-proof (induction ks)
-  case Nil thus ?case by simp
-next
-  case (Cons a as)
-  have "fold (\<lambda>k f. f(k := v)) (a # as) f = fold (\<lambda>k f. f(k := v)) as (f(a := v))" by simp
-  thus ?case
-  proof (cases "k \<in> set as")
-    case True
-    then show ?thesis sorry
-  next
-    case False
-    hence "fold (\<lambda>k f. f(k := v)) as f k = f k" using fold_upd_preserves by metis
-    then show ?thesis sorry
-  qed
-qed
+definition "g \<equiv> THE x. x = (5::nat) + 1"
+thm ex1_eq
+lemma "\<exists>! h. (5::nat) + 1 = h" sorry
 
-lemma
-  assumes "k \<notin> set keys"
-  shows "upd_all rel keys values k = rel k"
-  using assms
-proof (induction keys arbitrary: rel)
-  case (Cons a as)
-  hence "a \<noteq> k" using assms by auto
-  thus ?case using upd_all_cons assms Cons
-    by (metis fun_upd_idem_iff fun_upd_twist list.set_intros(2))
-qed (simp add: upd_all_def)
+lemma "\<exists>h. P h \<Longrightarrow> \<forall>a b. P a \<and> P b \<longrightarrow> a = b \<Longrightarrow> \<exists>!h. P h"
+  by blast
 
-  
+definition "d \<equiv> THE x. x > (5::nat)"
 
-lemma
-  assumes "k \<in> set keys"
-  shows "set (upd_all rel keys values k) = set (rel k) \<union> set values"
-  using assms
-proof (induction keys arbitrary: rel)
-  case (Cons a as)
-  have 1: "upd_all rel (a#as) values = upd_all (rel(a := conc_unique values (rel a))) as values"
-    by (simp add: upd_all_cons)
-  thus ?case
-  proof (cases "a = k")
-    case True
-    hence "upd_all rel (a#as) values k = conc_unique values (rel a)" using 1 sorry
-    then show ?thesis sorry
-  next
-    case False
-    then show ?thesis sorry
-  qed
-qed simp
+lemma "y = (THE x. P x) \<Longrightarrow> \<exists>!x. P x" oops
 
+(* random *)
 
-fun reach_aux :: "('a \<times> 'a) list \<Rightarrow> ('a \<Rightarrow> ('a list)) \<Rightarrow> ('a \<Rightarrow> ('a list)) \<Rightarrow> ('a \<Rightarrow> ('a list))" where
-  "reach_aux [] R L = L" |
-  "reach_aux ((l, r) # rest) R L = 
-    (let l_rs = R l; r_ls = L r in
-    reach_aux rest
-      (upd_all R r_ls l_rs)
-      (upd_all L l_rs r_ls))"
-
-fun reach_aux_aux :: "('a \<times> 'a) list \<Rightarrow> ('a \<times> 'a) list \<Rightarrow> ('a \<Rightarrow> ('a list)) \<Rightarrow> ('a \<Rightarrow> ('a list)) \<Rightarrow> ('a \<Rightarrow> ('a list))" where
-  "reach_aux_aux [] done R L = L" |
-  "reach_aux_aux ((l, r) # todo) done R L = 
-    (let l_rs = R l; r_ls = L r in
-    reach_aux_aux todo ((l, r) # done)
-      (upd_all R r_ls l_rs)
-      (upd_all L l_rs r_ls))"
-
-abbreviation reachable_nodes :: "('a \<times> 'a) list \<Rightarrow> 'a \<Rightarrow> ('a list)" where
-  "reachable_nodes rel \<equiv> reach_aux rel (\<lambda>x. [x]) (\<lambda>x. [x])"
-
-value "map (reachable_nodes [(1::nat, 0::nat),(2,0),(3,2),(4,2),(5,4),(5,3),(7,3),(6,5)]) [0, 1, 2, 3, 4, 5, 6, 7]"
-value "map (reachable_nodes ([(1, 0), (2, 0), (3, 1), (7, 6), (6, 5)]:: (nat\<times>nat) list)) [0, 1, 2, 3, 4, 5, 6, 7]"
-
-lemma "(x, x) \<in> rel\<^sup>*" by simp
-
-lemma reach_aux_aux: "reach_aux rel R L = reach_aux_aux rel dones R L"
-  apply (induction rel arbitrary: dones R L)
-  by auto
-
-definition describes_rel :: "('a \<times> 'a) set \<Rightarrow> ('a \<Rightarrow> 'a list) \<Rightarrow> bool" where
-  "describes_rel rel bags \<equiv> \<forall>x y. y \<in> set (bags x) \<longleftrightarrow> (x, y) \<in> rel"
-
-thm rtrancl_insert (* (insert (a, b) r)\<^sup>* = r\<^sup>* \<union> {(x, y). (x, a) \<in> r\<^sup>* \<and> (b, y) \<in> r\<^sup>*} *)
-
-
-
-lemma upd_all_L:
-  assumes "describes_rel (rel\<^sup>*) L"
-          "describes_rel ((rel\<^sup>*)\<inverse>) R"
-  shows "describes_rel (({(l, r)} \<union> rel)\<^sup>*) (upd_all L (R l) (L r))"
-  sorry
-
-lemma upd_all_R:
-  assumes "describes_rel (rel\<^sup>*) L"
-          "describes_rel ((rel\<^sup>*)\<inverse>) R"
-        shows "describes_rel ((({(l, r)} \<union> rel)\<^sup>*)\<inverse>) (upd_all R (L r) (R l))"
-proof -
-  from assms(2) have 1: "describes_rel ((rel\<inverse>)\<^sup>*) R" by (simp add: rtrancl_converse)
-  from assms(1) have 2: "describes_rel (((rel\<inverse>)\<^sup>*)\<inverse>) L" by (simp add: rtrancl_converse)
-  have 3: "describes_rel (({(r, l)} \<union> rel\<inverse>)\<^sup>*) (upd_all R (L r) (R l))"
-    by (rule upd_all_L[OF 1 2])
-  have "({(l, r)} \<union> rel)\<inverse> = {(r, l)} \<union> rel\<inverse>" by auto
-  moreover have   "(({(l, r)} \<union> rel)\<^sup>*)\<inverse> = (({(l, r)} \<union> rel)\<inverse>)\<^sup>*" by (simp add: rtrancl_converse)
-  ultimately have "(({(l, r)} \<union> rel)\<^sup>*)\<inverse> = ({(r, l)} \<union> rel\<inverse>)\<^sup>*" by simp
-  from 3 this show ?thesis by simp
-qed
-
-
-lemma reach_aux_aux_correct:
-  assumes "describes_rel ((set dones)\<^sup>*) L"
-          "describes_rel (((set dones)\<^sup>*)\<inverse>) R"
-  shows "describes_rel ((set todo \<union> set dones)\<^sup>*) (reach_aux_aux todo dones R L)"
-  using assms
-proof (induction todo arbitrary: dones L R)
-  case (Cons t todo)
-  let ?rel = "set dones"
-  obtain l r where lr: "t = (l, r)" by fastforce
-  note reach_aux_aux.simps(2)[unfolded Let_def] (* TODO how to have simp deal with "let" again? *)
-  hence aux_it: "reach_aux_aux ((l, r) # todo) dones R L =
-    reach_aux_aux todo ((l, r) # dones)
-      (upd_all R (L r) (R l))
-      (upd_all L (R l) (L r))" by simp
-  
-  have L: "describes_rel ((set ((l, r) # dones))\<^sup>*) (upd_all L (R l) (L r))"
-    using assms Cons.prems upd_all_L by simp
-  have R: "describes_rel (((set ((l, r) # dones))\<^sup>*)\<inverse>) (upd_all R (L r) (R l))"
-    using assms Cons.prems upd_all_R by simp
-  from L R have "describes_rel ((set todo \<union> set ((l, r) # dones))\<^sup>*)
-   (reach_aux_aux todo ((l, r) # dones) (upd_all R (L r) (R l)) (upd_all L (R l) (L r)))"
-    by (rule Cons.IH)
-  hence "describes_rel ((set (t # todo) \<union> set dones)\<^sup>*)
-    (reach_aux_aux (t # todo) dones R L)" using aux_it lr by simp
-  thus ?case .
-qed simp
-
-lemma "describes_rel ({}\<^sup>*) (\<lambda>x. [x])"
-  by (auto simp add: describes_rel_def)
-lemma "describes_rel (({}\<^sup>*)\<inverse>) (\<lambda>x. [x])"
-  by (auto simp add: describes_rel_def)
-
-lemma reach_aux_aux_usage:
-  shows "describes_rel ((set rel)\<^sup>*) (reach_aux_aux rel [] (\<lambda>x. [x]) (\<lambda>x. [x]))"
-proof -
-  have 1: "describes_rel ((set [])\<^sup>*) (\<lambda>x. [x])" by (auto simp add: describes_rel_def)
-  moreover have 2: "describes_rel (((set [])\<^sup>*)\<inverse>) (\<lambda>x. [x])" by (auto simp add: describes_rel_def)
-  moreover note reach_aux_aux_correct[OF 1 2]
-  ultimately show ?thesis by simp
-qed
-
-
-theorem reachable_iff_in_star: "describes_rel ((set rel)\<^sup>*) (reachable_nodes rel)"
-  using reach_aux_aux_usage reach_aux_aux
-  by metis
+definition foo :: "nat \<Rightarrow> [nat, nat] \<Rightarrow> nat" where
+  "foo a b c = a + b - c"
 
 
 
